SATsolver/Experiment/DPLL/completeness.lean
@@ -1,0 +1,129 @@
+import SATsolver.Experiment.Relations.Theories
+
+namespace Completenes
+
+theorem sat_eq_not_con_or_ud {t : Trail}{f : Formula}:
+  t.wf → (t ⊨ f ↔ ¬ (t ⊭ f ∨ t ¿ f)) := by
+  intro twf
+  simp[Satisfies.sat, Conflict.con, Undecided.ud]
+  constructor
+  case mp =>
+    intro call
+    constructor
+    case left =>
+      intro c cmem
+      obtain ⟨ l, lc, lt ⟩ := call c cmem
+      exists l
+      constructor
+      case left => exact lc
+      case right =>
+        intro contra
+        have := Trail.lit_and_litn_not_wf lt contra
+        contradiction
+    case right =>
+      intro c cmem l lmem hname
+      obtain ⟨ l, lc, lt ⟩ := call c cmem
+      exists l
+      constructor
+      case left => exact lc
+      case right =>
+        constructor
+        case left => exact Trail.mem_lits_mem_names lt
+        case right =>
+          intro contra
+          have := Trail.lit_and_litn_not_wf lt contra
+          contradiction
+  case mpr =>
+    intro h c cmem
+    obtain ⟨ l, lc, lt ⟩ := h.1 c cmem
+    have := h.2 c cmem l lc
+    by_cases lmem : l ∈ t.lits
+    case pos => exists l
+    case neg =>
+      have hname :¬l.name ∈ t.names := by
+        intro contra
+        rw[←Trail.mem_lits_names_eq] at contra
+        simp[lmem, lt] at contra
+      obtain ⟨ j, jmem, heq ⟩  := this hname
+      exists j
+      constructor
+      case left => exact jmem
+      case right =>
+        have := Trail.mem_lits_names_eq.mpr heq.1
+        simp[heq.2] at this
+        exact this
+
+
+theorem from_con {tl : Trail}{f : Formula} :
+  tl ⊭ f → ¬ ∃ hd, Trail.wf (hd++tl) ∧ hd ++tl ⊨ f := by
+  simp[Conflict.con, Satisfies.sat]
+  intro c cmem call hd hdwf
+  exists c
+  constructor
+  case left => exact cmem
+  case right =>
+    intro l lmem
+    have negmem := call l lmem
+    have lname : l.name ∈ Trail.names (hd++tl) := by
+      have := Trail.mem_lits_mem_names negmem
+      simp[Lit.name_name_negate] at this
+      simp[Trail.names] at this  ⊢
+      right; exact this
+    have := Trail.lit_of_wf lname hdwf
+    cases this
+    case inl lh =>
+      have := lh.2
+      have : l.negate ∈ (hd ++ tl).lits := by
+        simp[Trail.lits] at negmem ⊢
+        right; exact negmem
+      contradiction
+    case inr rh =>
+      exact rh.1
+
+
+theorem modifier {tl : Trail}{f : Formula}{a : ALit}:
+  (¬ ∃ hd, (hd++a::tl) ⊨ f) → (¬ ∃ hd, (hd++tl) ⊨ f) := by
+  simp
+  intro ah hd
+  have := ah hd
+  simp[Satisfies.sat] at this ⊢
+  obtain ⟨ c, cmem, call ⟩ := this
+  exists c
+  constructor
+  case left => exact cmem
+  case right =>
+    intro l lmem
+    have := call l lmem
+    simp[Trail.lits] at this ⊢
+    constructor
+    case left => exact this.1
+    case right => exact this.2.2
+
+def invariant (t : Trail)(f : Formula) : Prop :=
+  match t with
+  | [] => True
+  | (ALit.decided _)::tl => invariant tl f
+  | (ALit.deduced l)::tl => (¬ ∃ (hd : Trail), Trail.wf (hd++tl) ∧ (hd++tl) ⊨ f ∧ l.negate ∈ hd.lits) ∧ invariant tl f
+
+theorem cons {a : ALit}{t : Trail}{f : Formula}:
+  Completenes.invariant (a::t) f → Completenes.invariant t f := by
+  intro h
+  cases a
+  case decided l => simpa [invariant] using h
+  case deduced l => exact h.2
+
+theorem append {hd tl : Trail}{f : Formula}:
+  Completenes.invariant (hd++tl) f → Completenes.invariant tl f := by
+  intro h
+  induction hd
+  case nil => simpa using h
+  case cons x xs ih => exact ih (cons h)
+
+theorem helper {l : Lit}{tl : Trail}{f : Formula} :
+  Trail.wf ((ALit.deduced l)::tl) → invariant ((ALit.deduced l)::tl) f → (¬ ∃ hd, (hd++(ALit.deduced l)::tl) ⊨ f) → (¬ ∃ hd, Trail.wf (hd++tl) ∧ hd ++tl ⊨ f) := by
+  intro twf hinv h hd
+  have := modifier h
+  simp at this
+  obtain ⟨ hd, hdwf, hdsat ⟩ := hd
+  have := this hd
+  contradiction
